Make the size of uninit compute.

theories/typing/uninit.v
@@ -12,11 +12,27 @@ Section uninit.
   Global Instance uninit_1_send : Send uninit_1.
   Proof. iIntros (tid1 tid2 vl) "H". done. Qed.
 
-  Definition uninit (n : nat) : type :=
+  Definition uninit0 (n : nat) : type :=
     Π (replicate n uninit_1).
 
+  Lemma uninit0_sz n : ty_size (uninit0 n) = n.
+  Proof. induction n. done. simpl. by f_equal. Qed.
+
+  (* We redefine uninit as an alias of uninit0, so that the size
+     computes directly to [n] *)
+  Program Definition uninit (n : nat) : type :=
+    {| ty_size := n; ty_own := (uninit0 n).(ty_own);
+       ty_shr := (uninit0 n).(ty_shr) |}.
+  Next Obligation. intros. by rewrite ty_size_eq uninit0_sz. Qed.
+  Next Obligation. intros. by apply ty_share. Qed.
+  Next Obligation. intros. by apply ty_shr_mono. Qed.
+
   Global Instance uninit_copy n : Copy (uninit n).
-  Proof. apply product_copy, Forall_replicate, _. Qed.
+  Proof.
+    destruct (product_copy (replicate n uninit_1)) as [A B].
+      by apply Forall_replicate, _.
+    rewrite uninit0_sz in B. by split.
+  Qed.
 
   Global Instance uninit_send n : Send (uninit n).
   Proof. apply product_send, Forall_replicate, _. Qed.
@@ -24,14 +40,18 @@ Section uninit.
   Global Instance uninit_sync n : Sync (uninit n).
   Proof. apply product_sync, Forall_replicate, _. Qed.
 
-  Lemma uninit_sz n : ty_size (uninit n) = n.
-  Proof. induction n. done. simpl. by f_equal. Qed.
+  Lemma uninit_uninit0_eqtype E L n :
+    eqtype E L (uninit0 n) (uninit n).
+  Proof. apply equiv_eqtype; (split; first split)=>//=. apply uninit0_sz. Qed.
 
   Lemma uninit_product_eqtype E L ns :
     eqtype E L (uninit (foldr plus 0%nat ns)) (Π(uninit <$> ns)).
   Proof.
-    induction ns as [|n ns IH]. done. revert IH.
-    by rewrite /= /uninit replicate_plus prod_flatten_l -!prod_app=>->.
+    rewrite -uninit_uninit0_eqtype. etrans; last first.
+    { apply product_proper. eapply Forall2_fmap, Forall_Forall2, Forall_forall.
+      intros. by rewrite -uninit_uninit0_eqtype. }
+    induction ns as [|n ns IH]=>//=. revert IH.
+    by rewrite /= /uninit0 replicate_plus prod_flatten_l -!prod_app=>->.
   Qed.
   Lemma uninit_product_eqtype' E L ns :
     eqtype E L (Π(uninit <$> ns)) (uninit (foldr plus 0%nat ns)).
@@ -47,7 +67,7 @@ Section uninit.
     (uninit n).(ty_own) tid vl ⊣⊢ ⌜length vl = n⌝.
   Proof.
     iSplit.
-    - iIntros "?". rewrite -{2}(uninit_sz n). by iApply ty_size_eq.
+    - rewrite ty_size_eq. auto.
     - iInduction vl as [|v vl] "IH" forall (n).
       + iIntros "%". destruct n; done.
       + iIntros (Heq). destruct n; first done. simpl.
